some changes to indexing in Box

examples/crypto/cryptobox/Box.DH.fst
@@ -37,17 +37,24 @@ noeq type entry (i:id) =
 type log_t (i:id) (r:rid) = m_rref r (seq (entry i)) grows
 
 
-noeq type dh_pkey = 
-  | DH_pkey:  #pk_i:id -> #region:rid ->rawpk:dh_share -> log:log_t pk_i region -> dh_pkey
+noeq abstract type dh_pkey = 
+  | DH_pkey:  #pk_id:id -> #region:rid ->rawpk:dh_share -> log:log_t pk_id region -> dh_pkey
 
 
 noeq abstract type dh_skey =
-  | DH_skey: #sk_i:id -> rawsk:dh_exponent -> pk:dh_pkey{pk.pk_i=sk_i} -> dh_skey 
+  | DH_skey: #sk_id:id -> rawsk:dh_exponent -> pk:dh_pkey{pk.pk_id=sk_id} -> dh_skey 
 
-val get_index: dh_skey -> Tot(id)
-let get_index k = k.sk_i
+val sk_get_index: sk:dh_skey -> Tot (i:id{i = sk.sk_id})
+let sk_get_index k = k.sk_id
 
-val keygen: #i:id -> (parent:rid) -> ST (dh_pair:(k:dh_pkey{k.pk_i=i}) * (k:dh_skey{k.sk_i=i}))
+val pk_get_index: pk:dh_pkey -> Tot (i:id{i = pk.pk_id})
+let pk_get_index k = k.pk_id
+
+val pk_get_rawpk: pk:dh_pkey -> Tot (raw:dh_share{raw=pk.rawpk})
+let pk_get_rawpk pk =
+  pk.rawpk
+
+val keygen: #i:id -> (parent:rid) -> ST (dh_pair:(k:dh_pkey{k.pk_id=i}) * (k:dh_skey{k.sk_id=i}))
   (requires (fun h -> True))
   (ensures (fun h0 k h1 -> True
 //  let (pk,sk) = k in
@@ -74,34 +81,51 @@ type safe_log_append pk entry h0 h1 =
     /\ witnessed (at_least (Seq.length (m_sel h0 pk.log)) entry pk.log)
 
 (**
+   Helper function to look entries up in a log.
+*)
+val equal_share: sk_id:id -> pk_id:id -> dh_sh:dh_share -> e:entry sk_id -> Tot bool
+let equal_share sk_id pk_id dh_sh e =
+  match e with 
+  | DH_entry ent_i ent_share _ -> ent_i=pk_id && ent_share = dh_sh
+
+(**
    If we prf_odh is true, the output of this function is random, if both 
    share and exponent are honest.
 *)
 val prf_odh_snd: sk:dh_skey -> pk:dh_pkey -> ST (PlainDH.key)
   ( requires (fun _ -> True))
-  ( ensures (fun _ k _ -> Box.AE.get_index k = (pk.pk_i, sk.sk_i)
+  ( ensures (fun _ k _ -> 
+    (Box.AE.get_index k = (sk.sk_id, pk.pk_id)) || (Box.AE.get_index k = (pk.pk_id, sk.sk_id))
   ))
 let prf_odh_snd dh_snd_sk dh_rcv_pk =
-  let pk_id = dh_rcv_pk.pk_i in
-  let sk_id = dh_snd_sk.sk_i in
+  let pk_id = dh_rcv_pk.pk_id in
+  let sk_id = dh_snd_sk.sk_id in
   let i = pk_id, sk_id in
   let ae_honest_i = ae_honestST i in
   if ae_honest_i && prf_odh then
-    let k' = PlainDH.keygen i dh_rcv_pk.region in
-    write_at_end dh_rcv_pk.log (DH_entry sk_id dh_snd_sk.pk.rawpk k');
-    k'
+    let rcv_log = m_read dh_rcv_pk.log in
+    let snd_log = m_read dh_snd_sk.pk.log in
+    let rcv_entry = seq_find (equal_share pk_id sk_id dh_rcv_pk.rawpk) rcv_log in
+    let snd_entry = seq_find (equal_share sk_id pk_id dh_snd_sk.pk.rawpk) snd_log in
+    match rcv_entry with
+    | Some (DH_entry _ _ k') -> k'
+    | None -> 
+      match snd_entry with
+      | Some (DH_entry _ _ k') -> k'
+      | None -> 
+      let k' = PlainDH.keygen i dh_rcv_pk.region in
+      write_at_end dh_rcv_pk.log (DH_entry sk_id dh_snd_sk.pk.rawpk k');
+      write_at_end dh_snd_sk.pk.log (DH_entry pk_id dh_rcv_pk.rawpk k');
+      k'
   else
     let real_k = dh_exponentiate dh_rcv_pk.rawpk dh_snd_sk.rawsk in
     let k=PlainDH.coerce_key i dh_rcv_pk.region real_k in
     k
 
-val equal_share: sk_i:id -> pk_i:id -> dh_sh:dh_share -> e:entry sk_i -> Tot bool
-let equal_share sk_i pk_i dh_sh e =
-  match e with 
-  | DH_entry ent_i ent_share _ -> ent_i=pk_i && ent_share = dh_sh
 
 
-val prf_odh_rcv: #(sk_id:id) -> dh_sk:dh_skey{dh_sk.sk_i=sk_id} -> #(pk_id:id) -> dh_snd_pk:dh_pkey{dh_snd_pk.pk_i=pk_id} ->  St (k:PlainDH.key{AE.get_index k = (sk_id,pk_id)}
+
+val prf_odh_rcv: #(sk_id:id) -> dh_sk:dh_skey{dh_sk.sk_id=sk_id} -> #(pk_id:id) -> dh_snd_pk:dh_pkey{dh_snd_pk.pk_id=pk_id} ->  St (k:PlainDH.key{AE.get_index k = (sk_id,pk_id)}
 )
 let prf_odh_rcv #sk_id dh_rcv_sk #pk_id dh_snd_pk  =
   let honest_i = ae_honestST (sk_id, pk_id) in
@@ -112,10 +136,12 @@ let prf_odh_rcv #sk_id dh_rcv_sk #pk_id dh_snd_pk  =
     | Some (DH_entry _ _ k') -> k'
     | None -> 
       let i = sk_id,pk_id in
+      let k = PlainDH.keygen i dh_rcv_sk.pk.region in
+      k
 //      let i = sk_id,dishonestId() in
-      let raw_k = dh_exponentiate dh_snd_pk.rawpk dh_rcv_sk.rawsk in
-      admit ();
-      PlainDH.coerce_key i dh_rcv_sk.pk.region raw_k
+//      let raw_k = dh_exponentiate dh_snd_pk.rawpk dh_rcv_sk.rawsk in
+//      admit ();
+//      PlainDH.coerce_key i dh_rcv_sk.pk.region raw_k
   else
     let i =  sk_id,pk_id in
     let raw_k = dh_exponentiate dh_snd_pk.rawpk dh_rcv_sk.rawsk in
