examples/crypto/cryptobox/Box.Indexing.fst
@@ -11,6 +11,7 @@ module MM = MonotoneMap
 
 // Make these abstract!
 type id = UInt32.t
+assume Index_hasEq: hasEq id
 private type range = fun id -> bool
 private let inv (f:MM.map' id range) = True
 private let table = MM.alloc #root #id #range #inv 
@@ -23,7 +24,7 @@ let honest (i:id) =
 let dishonest (i:id) =
   MR.witnessed (MM.contains table i false)
 
-assume val lemma_dis_implies_not: i:id -> Lemma 
+val lemma_dis_implies_not: i:id -> Lemma 
   (requires (True))
   (ensures (dishonest i ==> ~(honest i)))
   [SMTPat (dishonest i) ]
@@ -34,50 +35,73 @@ let honestST (i:id) =
   MR.m_recall table;
   match MM.lookup table i with
   |Some v -> 
-    v=true
+    v
   |None -> 
-    MM.extend table i false;
-    false
+    MM.extend table i true;
+    true
 
 type ae_id = (id*id)
-private type ae_range = fun (i:ae_id) -> (b:bool{b ==> honest (fst i) /\ honest (snd i)})
-private let ae_inv (f:MM.map' ae_id ae_range) = True
-private let ae_table = MM.alloc #root #ae_id #ae_range #ae_inv 
 
+let ae_honest (i1,i2:ae_id) =
+  honest i1 /\ honest i2
 
+let ae_dishonest (i1,i2:ae_id) =
+  dishonest i1 \/ dishonest i2
 
-assume val generate_ae_id: i1:id -> i2:id -> Tot (i3:ae_id{i3=(i1,i2)})
+val ae_honestST: i:(id*id) -> St(b:bool{(b ==> (ae_honest i)) /\ (not b ==> (ae_dishonest i))})
+let ae_honestST (i1,i2) =
+  let h1 = honestST i1 in 
+  let h2 = honestST i2 in
+  h1 && h2
 
-
-//assume val ae_honest: i:ae_id -> Tot (b:bool{b ==> (honest (fst i) /\ honest (snd i))})
-let ae_honest (i:ae_id) =
-  honest (fst i) /\ honest (snd i) /\
-  MR.witnessed (MM.contains ae_table i true)
-
-let ae_dishonest (i:ae_id) =
-  dishonest (fst i) \/ dishonest (snd i) \/
-  MR.witnessed (MM.contains ae_table i false)
-
-assume val lemma_ae_dis_implies_not: i:ae_id -> Lemma 
+val lemma_ae_dis_implies_not: i:ae_id -> Lemma 
   (requires (True))
   (ensures (ae_dishonest i ==> ~(ae_honest i)))
-  [SMTPat (ae_dishonest i) ]
-  
-val ae_honestST: i:ae_id -> ST(b:bool{(b ==> ae_honest i) /\ (not b ==> ae_dishonest i)})
-  (requires (fun h0 -> True))
-  (ensures (fun h0 t h1 -> 
-    modifies (Set.singleton root) h0 h1 // precise enough?
-    ))
-let ae_honestST (i:ae_id) =
-  MR.m_recall ae_table;
-  match MM.lookup ae_table i with
-  |Some v -> 
-    v=true
-  |None -> 
-    MM.extend ae_table i false;
-    false
+  [SMTPat (ae_honest i) ]
 
 
-//val ae_honest: i:ae_id -> Tot (b:bool ==> (forall x. mem x i ==> honest x))
+val lemma_ae_hon_implies_not_dis: i:ae_id -> Lemma 
+  (requires (True))
+  (ensures (ae_honest i ==> ~(ae_dishonest i)))
+  [SMTPat (ae_honest i) ]
 
-assume Index_hasEq: hasEq id
+//private type ae_range = fun (i:ae_id) -> (b:bool{b ==> honest (fst i) /\ honest (snd i)})
+//private let ae_inv (f:MM.map' ae_id ae_range) = True
+//private let ae_table = MM.alloc #root #ae_id #ae_range #ae_inv 
+//
+//
+//
+//assume val generate_ae_id: i1:id -> i2:id -> Tot (i3:ae_id{i3=(i1,i2)})
+//
+//
+////assume val ae_honest: i:ae_id -> Tot (b:bool{b ==> (honest (fst i) /\ honest (snd i))})
+//let ae_honest (i:ae_id) =
+//  honest (fst i) /\ honest (snd i) /\
+//  MR.witnessed (MM.contains ae_table i true)
+//
+//let ae_dishonest (i:ae_id) =
+//  dishonest (fst i) \/ dishonest (snd i) \/
+//  MR.witnessed (MM.contains ae_table i false)
+//
+//assume val lemma_ae_dis_implies_not: i:ae_id -> Lemma 
+//  (requires (True))
+//  (ensures (ae_dishonest i ==> ~(ae_honest i)))
+//  [SMTPat (ae_dishonest i) ]
+//  
+//val ae_honestST: i:ae_id -> ST(b:bool{(b ==> ae_honest i) /\ (not b ==> ae_dishonest i)})
+//  (requires (fun h0 -> True))
+//  (ensures (fun h0 t h1 -> 
+//    modifies (Set.singleton root) h0 h1 // precise enough?
+//    ))
+//let ae_honestST (i:ae_id) =
+//  MR.m_recall ae_table;
+//  match MM.lookup ae_table i with
+//  |Some v -> 
+//    v=true
+//  |None -> 
+//    MM.extend ae_table i false;
+//    false
+//
+//
+////val ae_honest: i:ae_id -> Tot (b:bool ==> (forall x. mem x i ==> honest x))
+//
