examples/crypto/cryptobox/Box.PKAE.fst
@@ -40,10 +40,10 @@ type rid = FStar.Monotonic.Seq.rid
    that is used for the encryption/decryption. The secret key is abstract.
 *)
 noeq abstract type pkae_pkey (pk_id:id) =
-  | PKey: #region:rid -> dh_pk:dh_pkey{dh_pk.pk_i=pk_id} -> pkae_pkey pk_id
+  | PKey: #region:rid -> dh_pk:dh_pkey{DH.pk_get_index dh_pk=pk_id} -> pkae_pkey pk_id
 
 noeq abstract type pkae_skey (sk_id:id) =
-  | SKey: dh_sk:dh_skey -> pkae_pk:pkae_pkey sk_id -> pkae_skey sk_id
+  | SKey: dh_sk:dh_skey{DH.sk_get_index dh_sk=sk_id} -> pkae_pk:pkae_pkey sk_id -> pkae_skey sk_id
 
 val keygen: #(i:id) -> rid -> St (pkae_pkey i * pkae_skey i)
 let keygen #i (parent:rid) =
@@ -59,33 +59,26 @@ let keygen #i (parent:rid) =
 type c = DH.dh_share * AE.cipher //lbytes(PKE.ciphersize + AE.ciphersize)
 
 
-(**
-   For every new message we encrypt, we generate a new id. If that
-   id is honest (which is only possible if pke is idealized), then
-   we encrypt the protected_pkae_plain. Else we strip it of its 
-   protection and encrypt the plain representation.
-*)
-val encrypt: #(pk_i:id) -> #(eph_i:id)-> pkae_pkey pk_i -> p:protected_pkae_plain{PlainPKAE.get_index p = (pk_i,eph_i)} -> St c 
-let encrypt #pk_i #eph_i pk p =
-  let region = new_region pk.region in
-  let eph_dh_pk,eph_dh_sk = DH.keygen #eph_i region in
-  let k = prf_odh_snd eph_dh_sk pk.dh_pk in
-  let ae_i = pk_i,eph_i in
-  assert (DH.get_index eph_dh_sk = snd ae_i);
-  assert (pk.dh_pk.pk_i = fst ae_i);
-  assert (DH.get_index eph_dh_sk = eph_i);
-  assert (pk.dh_pk.pk_i = pk_i);
-  assert (ae_i = (pk_i,eph_i));
+val encrypt: #(pk_id:id) -> #(sk_id:id) -> pkae_pkey pk_id -> pkae_skey sk_id -> p:protected_pkae_plain{PlainPKAE.get_index p = (pk_id,sk_id)} -> St c 
+let encrypt #pk_id #sk_id pkae_pk  pkae_sk p =
+  let k = prf_odh_snd pkae_sk.dh_sk pkae_pk.dh_pk in
+  let ae_i = pk_id,sk_id in
+  assert(AE.get_index k = ae_i);
+//  assert (DH.get_index eph_dh_sk = snd ae_i);
+//  assert (pk.dh_pk.pk_i = fst ae_i);
+//  assert (DH.get_index eph_dh_sk = eph_i);
+//  assert (pk.dh_pk.pk_i = pk_i);
+//  assert (ae_i = (pk_i,eph_i));
   let ae_m = ae_message_wrap #ae_i p in
   //let dh_m = dh_message_wrap #pk.i eph_dh_pk.rawpk in
-  eph_dh_pk.rawpk,(AE.encrypt #ae_i k ae_m)
+  DH.pk_get_rawpk pkae_pk.dh_pk,(AE.encrypt #ae_i k ae_m)
 
 
-val decrypt: #(sk_i:id) -> pkae_skey sk_i -> #(pk_i:id) -> pkae_pkey sk_i -> c -> St(option (p:protected_pkae_plain//{PlainPKAE.get_index p = (sk_i,pk_i) }
+val decrypt: #(sk_id:id) -> pkae_skey sk_id -> #(pk_id:id) -> pkae_pkey sk_id -> c -> St(option (p:protected_pkae_plain//{PlainPKAE.get_index p = (sk_i,pk_i) }
 ))
-let decrypt #sk_i sk #pk_i pk c =
+let decrypt #sk_id sk #pk_id pk c =
   let (dh_sh,ae_c) = c in 
-  let k = prf_odh_rcv #sk_i sk.dh_sk #pk_i pk.dh_pk  in
+  let k = prf_odh_rcv #sk_id sk.dh_sk #pk_id pk.dh_pk  in
   let ae_i = AE.get_index k in
   (match AE.decrypt #ae_i k ae_c with
   | Some p -> 
