examples/crypto/HyE.Indexing.fst
@@ -1,0 +1,49 @@
+module HyE.Indexing
+
+open FStar.Seq
+
+module MM = MonotoneMap
+module HH = FStar.HyperHeap
+module HS = FStar.HyperStack
+module MR = FStar.Monotonic.RRef
+module MS = FStar.Monotonic.Seq
+
+type pke_id = MR.rid
+type ae_id = pke_id*UInt32.t
+
+type ae_id_table (r:pke_id) = MR.m_rref r (seq UInt32.t) MS.grows
+
+
+type pke_id_to_ae_ids = fun (pk_id:pke_id) -> (ae_id_table pk_id)
+
+
+let trivial_invariant (m:MM.map' pke_id pke_id_to_ae_ids)  = True
+
+
+abstract let table_region: MR.rid = new_region HH.root
+let pke_ae_id_table: MM.t table_region pke_id pke_id_to_ae_ids trivial_invariant = 
+  MM.alloc #table_region #pke_id #pke_id_to_ae_ids #trivial_invariant
+
+
+// Do lookups in the global table here
+val pke_honest: pke_id -> MR.rid -> GTot Type0
+let pke_honest pk_id h =
+  MR.witnessed (MM.defined pke_ae_id_table pk_id)
+  
+
+val ae_honest: k_id:ae_id -> h:MR.rid -> GTot (b:Type0)//{b ==> pke_honest (fst k_id) h})
+let ae_honest k_id h =
+  MR.witnessed (MR.rid_exists (fst k_id)) /\
+  pke_honest (fst k_id) h /\
+  MR.witnessed (MM.contains (fst k_id) k_id)
+
+val fresh_pke_id: unit -> Tot (i:pke_id{pke_honest i})
+val is_fresh_pke_id: pke_id -> HS.mem-> GTot bool
+let is_fresh_pke_id pk_id h =
+  MM.sel (MR.m_sel h pke_ae_id_table) pk_id = None
+
+// TODO: Try typechecking without refinements!
+val fresh_ae_id: pk_id:pke_id -> Tot (k_id:ae_id{fst k_id = pk_id /\ (pke_honest pk_id ==> b2t (ae_honest k_id))})
+val dishonest_ae_id: pk_id:pke_id -> Tot (k_id:ae_id{not (ae_honest k_id) && fst k_id = pk_id})
+
+assume Index_hasEq: hasEq pke_id
